refactoring `TaskM`

Mt/Task/Impl.lean
@@ -3,48 +3,46 @@ import Mt.Reservation
 namespace Mt.TaskM.impl
 
 inductive IterationResult (spec : Spec) (T : Type)
-| Done : spec.Reservation -> spec.State -> T -> IterationResult spec T
-| Panic : spec.Reservation -> spec.State -> String -> IterationResult spec T
-| Running : spec.Reservation -> spec.State -> 
-    (spec.Reservation -> Bool) ->
-    (spec.Reservation -> spec.State -> IterationResult spec T) ->
+| Done : spec.State -> T -> IterationResult spec T
+| Panic : spec.State -> String -> IterationResult spec T
+| Running : spec.State -> (spec.State -> Bool) ->
+    (spec.State -> IterationResult spec T) ->
     IterationResult spec T
 
-def TaskM (spec : Spec) (T : Type) :=spec.Reservation -> spec.State -> IterationResult spec T
+def TaskM (spec : Spec) (T : Type) :=spec.State -> IterationResult spec T
 
 namespace TaskM
 
 variable {spec : Spec}
 
 def atomic_read_modify_read
-  (f : spec.Reservation -> spec.State -> T × spec.Reservation × spec.State)
+  (f : spec.State -> T × spec.State)
   : TaskM spec T
-| r, s => match f r s with
-  | ⟨t, r', s'⟩ => IterationResult.Done r' s' t
+| s => match f s with
+  | ⟨t, s'⟩ => IterationResult.Done s' t
 
 def panic {T : Type} (msg : String) : TaskM spec T
-| r, s => IterationResult.Panic r s msg
+| s => IterationResult.Panic s msg
 
 def atomic_assert
   (cond : spec.State -> Bool)
   : TaskM spec Unit
-| r, s => if cond s then
-    IterationResult.Done r s ⟨⟩
+| s => if cond s then
+    IterationResult.Done s ⟨⟩
   else
-    IterationResult.Panic r s "Assertion failed"
+    IterationResult.Panic s "Assertion failed"
 
 def atomic_blocking_rmr
-  (block_until : spec.Reservation -> Bool)
-  (f : spec.Reservation -> spec.State -> T × spec.Reservation × spec.State)
-  : TaskM spec T
-| r, s => IterationResult.Running r s block_until (atomic_read_modify_read f)
+  (block_until : spec.State -> Bool)
+  (f : spec.State -> T × spec.State) : TaskM spec T
+| s => IterationResult.Running s block_until (atomic_read_modify_read f)
 
 inductive is_direct_cont {T : Type} : TaskM spec T -> TaskM spec T -> Prop
 | running
     {p cont : TaskM spec T}
-    {r r' s s'}
-    {block_until : spec.Reservation -> Bool}
-    (iteration : p r s = IterationResult.Running r' s' block_until cont)
+    {s s'}
+    {block_until : spec.State -> Bool}
+    (iteration : p s = IterationResult.Running s' block_until cont)
     : is_direct_cont cont p
 
 theorem is_direct_cont.wf {T : Type} : WellFounded (@is_direct_cont spec T) :=by
@@ -53,64 +51,62 @@ theorem is_direct_cont.wf {T : Type} : WellFounded (@is_direct_cont spec T) :=by
   constructor
   intro cont is_cont
   cases is_cont
-  rename_i r r' s s' bu iteration
-  exact helper (p r s) cont iteration
+  rename_i s s' bu iteration
+  exact helper (p s) cont iteration
 
 where
-  helper (it : IterationResult spec T) (p : TaskM spec T) {r s block_until} :
-    it = IterationResult.Running r s block_until p → Acc is_direct_cont p :=by
-    revert p r s block_until
+  helper (it : IterationResult spec T) (p : TaskM spec T) {s block_until} :
+    it = IterationResult.Running s block_until p → Acc is_direct_cont p :=by
+    revert p s block_until
     induction it
     . intros ; contradiction
     . intros ; contradiction
-    . intro p r s bu h
-      rename_i r' s' bu' p' IH
+    . intro p s bu h
+      rename_i s' bu' p' IH
       injection h ; rename_i h ; rw [h] at IH
       constructor
       intro cont is_cont ; cases is_cont ; rename_i h
-      exact IH _ _ _ h
+      exact IH _ _ h
 
 instance instWf {T : Type} : WellFoundedRelation (TaskM spec T) where
   rel :=is_direct_cont
   wf  :=is_direct_cont.wf
 
 def pure {T : Type} (t : T) : TaskM spec T :=
-  λ r s => IterationResult.Done r s t
+  λ s => IterationResult.Done s t
 
 def bind {U V : Type} (mu : TaskM spec U) (f : U -> TaskM spec V) : TaskM spec V :=
-  λ r s => match h : mu r s with
-    | IterationResult.Done r' s' u => IterationResult.Running r' s' (λ _ => true) (f u)
-    | IterationResult.Panic r' s' msg => IterationResult.Panic r' s' msg
-    | IterationResult.Running r' s' block_until cont =>
+  λ s => match h : mu s with
+    | IterationResult.Done s' u => IterationResult.Running s' (λ _ => true) (f u)
+    | IterationResult.Panic s' msg => IterationResult.Panic s' msg
+    | IterationResult.Running s' block_until cont =>
         have : is_direct_cont cont mu :=⟨h⟩
-        IterationResult.Running r' s' block_until (bind cont f)
+        IterationResult.Running s' block_until (bind cont f)
 termination_by bind => mu
 
 theorem bind_def {U V spec}
   {mu : TaskM spec U} {f : U -> TaskM spec V}
-  {r s}
-  : (bind mu f) r s = match mu r s with
-    | IterationResult.Done r' s' u => IterationResult.Running r' s' (λ _ => true) (f u)
-    | IterationResult.Panic r' s' msg => IterationResult.Panic r' s' msg
-    | IterationResult.Running r' s' block_until cont =>
-        IterationResult.Running r' s' block_until (bind cont f) :=by
+  {s}
+  : (bind mu f) s = match mu s with
+    | IterationResult.Done s' u => IterationResult.Running s' (λ _ => true) (f u)
+    | IterationResult.Panic s' msg => IterationResult.Panic s' msg
+    | IterationResult.Running s' block_until cont =>
+        IterationResult.Running s' block_until (bind cont f) :=by
   simp only [bind]
-  cases mu r s <;> rfl
+  cases mu s <;> rfl
 
 theorem bind_assoc {U V W : Type}
   (mu : TaskM spec U)
   (f : U -> TaskM spec V)
   (g : V -> TaskM spec W) :
   mu.bind (fun u => (f u).bind g) = (mu.bind f).bind g :=by
-  apply funext ; intro reservation0
   apply funext ; intro s0
   simp only [bind_def]
-  induction mu reservation0 s0 <;> try rfl
-  rename_i r' s' block_until cont IH
+  induction mu s0 <;> try rfl
+  rename_i s' block_until cont IH
   simp only []
   simp only [<- bind_def] at IH
-  apply congrArg (IterationResult.Running _ _ _)
-  apply funext ; intro r
+  apply congrArg (IterationResult.Running _ _)
   apply funext ; intro s
   exact IH ..
 
